src/Std/Data/DHashMap/Internal/Defs.lean
@@ -227,6 +227,43 @@ where
     expandIfNecessary ⟨⟨size', buckets'⟩, by simpa [buckets']⟩
 
 /-- Internal implementation detail of the hash map -/
+@[inline] def alter [BEq α] [Hashable α] [LawfulBEq α] (m : Raw₀ α β) (a : α)
+    (f : Option (β a) → Option (β a)) : Raw₀ α β :=
+  let ⟨⟨size, buckets⟩, hm⟩ := m
+  let ⟨i, h⟩ := mkIdx buckets.size hm (hash a)
+  let bkt := buckets[i]
+  if bkt.contains a then
+    let buckets' := buckets.uset i .nil h
+    let (bkt', some?) := bkt.alter' a f
+    let size' := if some? then size else size - 1
+    ⟨⟨size', buckets'.uset i bkt' (by simpa [buckets'])⟩, by simpa [buckets']⟩
+  else
+    match f none with
+    | none => m
+    | some b =>
+      let size'    := size + 1
+      let buckets' := buckets.uset i (.cons a b bkt) h
+      expandIfNecessary ⟨⟨size', buckets'⟩, by simpa [buckets']⟩
+
+def alterAux [BEq α] [Hashable α] [LawfulBEq α] (m : Raw₀ α β) (a : α)
+  (f : Option (β a) → Option (β a)) : Raw₀ α β :=
+let ⟨⟨size, buckets⟩, hm⟩ := m
+let ⟨i, h⟩ := mkIdx buckets.size hm (hash a)
+let bkt := buckets[i]
+if bkt.contains a then
+  let buckets' := buckets.uset i .nil h
+  let (bkt', some?) := bkt.alter' a f
+  let size' := if some? then size else size - 1
+  ⟨⟨size', buckets'.uset i bkt' (by simpa [buckets'])⟩, by simpa [buckets']⟩
+else
+  match f none with
+  | none => m
+  | some b =>
+    let size'    := size + 1
+    let buckets' := buckets.uset i (.cons a b bkt) h
+    expandIfNecessary ⟨⟨size', buckets'⟩, by simpa [buckets']⟩
+
+/-- Internal implementation detail of the hash map -/
 @[inline] def containsThenInsert [BEq α] [Hashable α] (m : Raw₀ α β) (a : α) (b : β a) :
     Bool × Raw₀ α β :=
   let ⟨⟨size, buckets⟩, hm⟩ := m
