src/Std/Data/DHashMap/Internal/Model.lean
@@ -310,6 +310,23 @@ def eraseₘaux [BEq α] [Hashable α] (m : Raw₀ α β) (a : α) : Raw₀ α �
 def eraseₘ [BEq α] [Hashable α] (m : Raw₀ α β) (a : α) : Raw₀ α β :=
   if m.containsₘ a then m.eraseₘaux a else m
 
+def alterₘ [BEq α] [Hashable α] [LawfulBEq α] (m : Raw₀ α β) (a : α)
+    (f : Option (β a) → Option (β a)) :
+    Raw₀ α β :=
+  if h : m.containsₘ a then
+    let b := m.get a h
+    match f (some b) with
+    | none => m.eraseₘ a
+    | some b' => m.replaceₘ a b'
+  else
+    match f none with
+    | none => m
+    | some b' => m.insertₘ a b'
+  -- let v := m.get?ₘ a
+  -- match f v with
+  -- | none => m.eraseₘ a
+  -- | some b => m.insertₘ a b
+
 /-- Internal implementation detail of the hash map -/
 def filterMapₘ (m : Raw₀ α β) (f : (a : α) → β a → Option (δ a)) : Raw₀ α δ :=
   ⟨withComputedSize (updateAllBuckets m.1.buckets fun l => l.filterMap f), by simpa using m.2⟩
@@ -390,6 +407,136 @@ theorem insert_eq_insertₘ [BEq α] [Hashable α] (m : Raw₀ α β) (a : α) (
     rw [Array.set_set, updateBucket]
     simp only [Array.uset, Array.ugetElem_eq_getElem]
   · rfl
+
+def alterAux [BEq α] [Hashable α] [LawfulBEq α] (m : Raw₀ α β) (a : α)
+    (f : Option (β a) → Option (β a)) : Raw₀ α β :=
+  let ⟨⟨size, buckets⟩, hm⟩ := m
+  let ⟨i, h⟩ := mkIdx buckets.size hm (hash a)
+  let bkt := buckets[i]
+  if m.containsₘ a then
+    let buckets' := buckets.uset i .nil h
+    let (bkt', some?) := bkt.alter' a f
+    let size' := if some? then size else size - 1
+    ⟨⟨size', buckets'.uset i bkt' (by simpa [buckets'])⟩, by simpa [buckets']⟩
+  else
+    match f none with
+    | none => m
+    | some b =>
+      let size'    := size + 1
+      let buckets' := buckets.uset i (.cons a b bkt) h
+      expandIfNecessary ⟨⟨size', buckets'⟩, by simpa [buckets']⟩
+
+theorem alter_eq_alterAux [BEq α] [Hashable α] [LawfulBEq α] (m : Raw₀ α β) (a : α)
+    (f : Option (β a) → Option (β a)) :
+    m.alter a f = alterAux m a f := by
+  rfl
+
+theorem alter_eq_eraseₘ [BEq α] [Hashable α] [LawfulBEq α] (m : Raw₀ α β) (a : α)
+    (f : Option (β a) → Option (β a)) (h₁ : m.containsₘ a) (h₂ : f (m.get?ₘ a) = none) :
+    m.alter a f = m.eraseₘ a := by
+  rw [alter_eq_alterAux]
+  unfold alterAux
+  simp only [h₁, reduceIte, Array.ugetElem_eq_getElem, Array.uset, Array.set_set]
+  congr
+  · split
+    · next hh =>
+      simp only [AssocList.alter'_snd, AssocList.getCast?_eq] at hh
+      simp only [get?ₘ, bucket, Array.ugetElem_eq_getElem, AssocList.getCast?_eq] at h₂
+      rw [h₂] at hh
+      contradiction
+    · rw [h₁]
+      dsimp [instDecidableEqBool, Bool.decEq, eraseₘaux]
+  · rw [h₁]
+    dsimp [instDecidableEqBool, Bool.decEq, eraseₘaux, updateBucket]
+    rw [AssocList.alter'_eq_of_contains]
+    split
+    · rfl
+    · next heq =>
+      dsimp [get?ₘ, bucket] at h₂
+      rw [AssocList.getCast?_eq] at h₂
+      rw [AssocList.getCast_eq] at heq
+      rw [← getValueCast?_eq_some_getValueCast] at heq
+      rw [h₂] at heq
+      contradiction
+      exact h₁
+
+theorem alter_eq_insertₘ [BEq α] [Hashable α] [LawfulBEq α] (m : Raw₀ α β) (a : α)
+    (f : Option (β a) → Option (β a)) (h₁ : ¬(m.containsₘ a)) (h₂ : (f (m.get?ₘ a)).isSome) :
+    m.alter a f = m.insertₘ a ((f (m.get?ₘ a)).get h₂) := by
+  rw [alter_eq_alterAux]
+  dsimp [alterAux, insertₘ]
+  dsimp [Option.isSome, get?ₘ] at h₂
+  unfold AssocList.getCast? at h₂
+  dsimp [containsₘ] at h₁
+  unfold AssocList.contains at h₁
+  simp only [ite_cond_eq_false _ _ (by simp only [eq_iff_iff, iff_false]; exact h₁)] at *
+  sorry
+
+theorem alter_eq_alterₘ [BEq α] [Hashable α] [LawfulBEq α] (m : Raw₀ α β) (a : α)
+    (f : Option (β a) → Option (β a)) :
+    m.alter a f = m.alterₘ a f := by
+  rw [alter, alterₘ]
+  dsimp
+  apply Eq.symm
+  split
+  · next h =>
+    have h' := h
+    dsimp [containsₘ, bucket] at h'
+    simp only [h', if_true]
+    rw [AssocList.alter'_snd]
+    simp only [Raw₀.get]
+    split
+    · next hnone =>
+      unfold eraseₘ eraseₘaux
+      simp [h]
+      apply And.intro
+      · rw [getValueCast?_eq_some_getValueCast]
+        simp only [Array.ugetElem_eq_getElem, AssocList.getCast_eq] at hnone
+        rw [hnone]
+        rfl
+      · unfold updateBucket
+        dsimp
+        unfold AssocList.alter'
+
+    · done
+  · next h =>
+    done
+  unfold containsₘ bucket
+  dsimp only [Array.ugetElem_eq_getElem, Array.uset]
+  split
+  · match f (some (m.get a _)) with
+    | .none =>
+      dsimp
+      split
+      · next h =>
+        unfold AssocList.alter' at h
+        split at h
+        · split at h
+          · contradiction
+          · simp only [Array.set_set]
+
+        · split at h
+          · dsimp at h
+            split at h
+            · contradiction
+            · done
+          · split at h
+            · done
+            · done
+      · congr
+        · done
+        · done
+    | .some _ => done
+    -- ext ; dsimp only
+    -- congr
+    -- · unfold AssocList.alter'
+    --   done
+    -- rw [AssocList.alter'_eq_of_contains]
+    -- unfold Raw₀.get
+    -- dsimp
+    -- simp
+  · done
+
 
 theorem containsThenInsert_eq_insertₘ [BEq α] [Hashable α] (m : Raw₀ α β) (a : α) (b : β a) :
     (m.containsThenInsert a b).2 = m.insertₘ a b := by
