src/Std/Data/DHashMap/Internal/AssocList/Lemmas.lean
@@ -146,6 +146,49 @@ theorem toList_replace [BEq α] {l : AssocList α β} {a : α} {b : β a} :
   · next k v t ih => cases h : k == a <;> simp_all [replace, List.replaceEntry_cons]
 
 @[simp]
+theorem alter'_eq_of_contains [BEq α] [LawfulBEq α] {l : AssocList α β} {a : α}
+    {f : Option (β a) → Option (β a)} (h : l.contains a) :
+    l.alter' a f = match f (l.getCast a h) with
+    | none => (l.erase a, false)
+    | some b => (l.replace a b, true) := by
+  generalize l = l, h = h
+  induction l
+  · contradiction
+  · next a' x xs ih =>
+      unfold contains at h
+      if heq : a' == a then
+        cases eq_of_beq heq
+        simp [alter', replace, erase, getValueCast]
+        rfl
+      else
+        unfold alter'
+        rw [Bool.not_eq_true] at heq
+        simp only [heq, Bool.false_eq_true, reduceDIte, getCast_eq, toList_cons, beq_iff_eq,
+          getValueCast, Option.some_get]
+        unfold getValueCast? erase replace
+        simp only [heq, Bool.false_eq_true, reduceDIte, cond_false]
+        simp only [Bool.or_eq_true, beq_iff_eq, beq_eq_false_iff_ne, ne_eq] at h heq
+        cases h <;> try contradiction
+        rw [ih (by assumption), getCast_eq, getValueCast, Option.some_get]
+        cases f (getValueCast? a xs.toList) <;> simp
+
+theorem alter'_snd [BEq α] [LawfulBEq α] {l : AssocList α β} {a : α}
+    {f : Option (β a) → Option (β a)} :
+    (l.alter' a f).snd = (f (l.getCast? a)).isSome := by
+  induction l
+  · unfold alter'
+    simp only [decide_false, decide_true, getCast?_eq, toList_nil, getValueCast?_nil]
+    cases f none <;> rfl
+  · next k v l ih =>
+    unfold alter'
+    simp only [beq_iff_eq, decide_false, decide_true, getCast?_eq, toList_cons]
+    unfold getValueCast?
+    split
+    · split <;> { next h => rw [h] ; rfl }
+    · rw [ih]
+      simp
+
+@[simp]
 theorem toList_erase [BEq α] {l : AssocList α β} {a : α} :
     (l.erase a).toList = eraseKey a l.toList := by
   induction l
